Towards executable model checker for simple network language including glue code

Simple_Networks/Simple_Network_Language_Export_Code.thy
@@ -1,5 +1,8 @@
 theory Simple_Network_Language_Export_Code
-  imports Simple_Network_Language_Renaming
+  imports
+    Simple_Network_Language_Renaming
+    "../UPPAAL_State_Networks_Impl_Refine_Calc"
+    "../library/Error_Monad"
 begin
 
 datatype result =
@@ -7,17 +10,61 @@ datatype result =
 
 abbreviation "renum_automaton \<equiv> Simple_Network_Rename_Defs.renum_automaton"
 
+hide_const m
+
+locale Simple_Network_Rename_Formula_String =
+  Simple_Network_Rename_Defs where automata = automata for automata ::
+    "(String.literal list \<times>
+     (String.literal act, String.literal, String.literal, int, String.literal, int) transition list
+      \<times> (String.literal \<times> (String.literal, int) cconstraint) list) list" +
+  assumes renum_states_inj:
+    "\<forall>i<n_ps. \<forall>x\<in>loc_set. \<forall>y\<in>loc_set. renum_states i x = renum_states i y \<longrightarrow> x = y"
+  and renum_clocks_inj: "inj_on renum_clocks clk_set'"
+  and renum_vars_inj:   "inj_on renum_vars var_set"
+  and bounds'_var_set: "fst ` set bounds' \<subseteq> var_set"
+  and loc_set_invs: "\<Union> ((\<lambda>g. fst ` set g) ` set (map (snd o snd) automata)) \<subseteq> loc_set"
+  and loc_set_broadcast: "\<Union> ((set o fst) ` set automata) \<subseteq> loc_set"
+  fixes \<Phi> :: "(String.literal, String.literal, int) formula"
+    and s\<^sub>0 :: "(String.literal \<times> int) list"
+    and L\<^sub>0 :: "String.literal list"
+  assumes L\<^sub>0_states: "L\<^sub>0 \<in> states"
+      and s\<^sub>0_dom: "fst ` set s\<^sub>0 = var_set" and s\<^sub>0_distinct: "distinct (map fst s\<^sub>0)"
+  assumes formula_dom:
+    "set1_formula \<Phi> \<subseteq> loc_set"
+    "locs_of_formula \<Phi> \<subseteq> {0..<n_ps}"
+    "vars_of_formula \<Phi> \<subseteq> var_set"
+begin
+
+interpretation Simple_Network_Rename_Formula
+  by (standard; 
+      rule renum_states_inj renum_clocks_inj renum_vars_inj bounds'_var_set
+      loc_set_invs loc_set_broadcast infinite_literal
+      L\<^sub>0_states s\<^sub>0_dom s\<^sub>0_distinct formula_dom)
+
+lemmas Simple_Network_Rename_intro = Simple_Network_Rename_Formula_axioms
+
+end
+
+definition rename_network where
+  "rename_network broadcast bounds' automata renum_acts renum_vars renum_clocks renum_states \<equiv>
+  let
+    automata = map_index (renum_automaton renum_acts renum_vars renum_clocks renum_states) automata;
+    broadcast = map renum_acts broadcast;
+    bounds' = map (\<lambda>(a,b,c). (renum_vars a, b, c)) bounds'
+  in
+    (broadcast, automata, bounds')
+"
+
 definition rename_mc where
   "rename_mc broadcast bounds' automata k L\<^sub>0 s\<^sub>0 formula
     m num_states num_actions renum_acts renum_vars renum_clocks renum_states
 \<equiv>
 let
    renaming_valid =
-    Simple_Network_Rename_Formula
+    Simple_Network_Rename_Formula_String
       broadcast bounds' renum_vars renum_clocks renum_states automata formula s\<^sub>0 L\<^sub>0;
-   automata = map_index (renum_automaton renum_acts renum_vars renum_clocks renum_states) automata;
-   broadcast = map renum_acts broadcast;
-   bounds' = map (\<lambda>(a,b,c). (renum_vars a, b, c)) bounds';
+   (broadcast, automata, bounds') = rename_network
+      broadcast bounds' automata renum_acts renum_vars renum_clocks renum_states;
    formula = map_formula renum_states renum_vars id formula;
    L\<^sub>0 = map_index renum_states L\<^sub>0;
    s\<^sub>0 = map (\<lambda>(x, v). (renum_vars x, v)) s\<^sub>0
@@ -57,13 +104,22 @@ theorem model_check_rename:
         (map_formula renum_states renum_vars id formula))
     >\<^sub>t"
 proof -
+  have *: "
+    Simple_Network_Rename_Formula_String
+        broadcast bounds renum_vars renum_clocks renum_states automata formula s\<^sub>0 L\<^sub>0
+  = Simple_Network_Rename_Formula
+        broadcast bounds renum_vars renum_clocks renum_states automata formula s\<^sub>0 L\<^sub>0
+  "
+    unfolding
+      Simple_Network_Rename_Formula_String_def Simple_Network_Rename_Formula_def
+      Simple_Network_Rename_def Simple_Network_Rename_Formula_axioms_def
+    using infinite_literal by auto
   define A where "A \<equiv> N broadcast automata bounds"
   define check where "check \<equiv> A,(L\<^sub>0, map_of s\<^sub>0, \<lambda>_ . 0) \<Turnstile> formula"
   define A' where "A' \<equiv> N
     (map renum_acts broadcast)
     (map_index (renum_automaton renum_acts renum_vars renum_clocks renum_states) automata)
-    (map (\<lambda>(a,b,c). (renum_vars a, b, c)) bounds)
-  "
+    (map (\<lambda>(a,b,c). (renum_vars a, b, c)) bounds)"
   define check' where "check' \<equiv>
     A',(map_index renum_states L\<^sub>0, map_of (map (\<lambda>(x, v). (renum_vars x, v)) s\<^sub>0), \<lambda>_ . 0) \<Turnstile>
     map_formula renum_states renum_vars id formula"
@@ -100,7 +156,7 @@ proof -
     simplified
     ]
   show ?thesis
-    unfolding rename_mc_def
+    unfolding rename_mc_def rename_network_def *
     unfolding
       A_def[symmetric] check_def[symmetric]
       preconds_sat_def[symmetric] renaming_valid_def[symmetric]
@@ -155,7 +211,7 @@ export_code precond_mc in SML module_name Test
 paragraph \<open>Code Setup for Renaming\<close>
 
 lemmas [code] =
-  Simple_Network_Rename_def
+  Simple_Network_Rename_Formula_String_def
   Simple_Network_Impl.clk_set'_def
   Simple_Network_Impl.clkp_set'_def
 
@@ -180,11 +236,259 @@ lemmas [code_unfold] =
   setcompr_eq_image
   Simple_Network_Impl.length_automata_eq_n_ps[symmetric]
 
-lemmas [code] =
-  Simple_Network_Rename_Formula_def
-  Simple_Network_Rename_Formula_axioms_def
-
-
 export_code rename_mc in SML module_name Test
+
+
+
+paragraph \<open>Calculating the Clock Ceiling\<close>
+
+context Simple_Network_Impl_nat_defs
+begin
+
+definition "clkp_inv i l \<equiv>
+  (UNION (set (filter (\<lambda> (a, b). a = l) (snd (snd (automata ! i))))) (collect_clock_pairs o snd))"
+
+definition "clkp_set'' i l \<equiv>
+    clkp_inv i l \<union> (\<Union> (l, g, _) \<in> set (fst (snd (automata ! i))). collect_clock_pairs g)"
+
+definition
+  "collect_resets i l = (\<Union> (l, g, a, f, r, _) \<in> set (fst (snd (automata ! i))). set r)"
+
+context
+  fixes q c :: nat
+begin
+
+  definition "n \<equiv> num_states q"
+
+  definition "V \<equiv> \<lambda> v. v \<le> m"
+
+  definition "
+    bound_g l \<equiv>
+      Max ({0} \<union> \<Union> ((\<lambda> (x, d). if x = c then {d} else {}) ` clkp_set'' q l))
+    "
+
+  definition "
+    bound_inv l \<equiv>
+      Max ({0} \<union> \<Union> ((\<lambda> (x, d). if x = c then {d} else {}) ` clkp_inv q l))
+  "
+
+  definition "
+    bound l \<equiv> max (bound_g l) (bound_inv l)
+  "
+
+definition "
+  resets l \<equiv>
+    let reset = collect_resets q l in
+    fold
+    (\<lambda> (l1, g, a, f, r, l') xs. if l1 \<noteq> l \<or> l' \<in> set xs \<or> c \<in> reset then xs else (l' # xs))
+    (fst (snd (automata ! q)))
+    []
+"
+
+text \<open>
+  Edges in the direction nodes to single sink.
+\<close>
+definition "
+  E' l \<equiv> resets l
+"
+
+text \<open>
+  Turning around the edges to obtain a single source shortest paths problem.
+\<close>
+(* XXX Tune for efficiency *)
+definition "
+  E l \<equiv> if l = n then [0..<n_ps] else filter (\<lambda> l'. l \<in> set (E' l')) [0..<n_ps]
+"
+
+text \<open>
+  Weights already turned around.
+\<close>
+definition "
+  W l l' \<equiv> if l = n then - bound l' else 0
+"
+
+definition "
+  G \<equiv> \<lparr> gi_V = V, gi_E = E, gi_V0 = [n], \<dots> = W \<rparr>
+"
+
+definition "
+  local_ceiling \<equiv>
+  let
+    w = calc_shortest_scc_paths G n
+  in
+    map (\<lambda> x. case x of None \<Rightarrow> 0 | Some x \<Rightarrow> nat(-x)) w
+"
+
+end
+
+definition "
+  k \<equiv>
+    rev $
+    fold
+      (\<lambda> q xs.
+        (\<lambda> x. rev x # xs) $
+        fold
+          (\<lambda> l xs.
+            (\<lambda> x. (0 # rev x) # xs) $
+            fold
+              (\<lambda> c xs. local_ceiling q c ! l # xs)
+              [1..<Suc m]
+              []
+          )
+          [0..<n q]
+          []
+      )
+      [0..<p]
+      []
+"
+
+end
+
+
+lemmas [code] =
+  Simple_Network_Impl_nat_defs.k_def
+  Simple_Network_Impl_nat_defs.local_ceiling_def
+  Simple_Network_Impl_nat_defs.n_def
+  Simple_Network_Impl_nat_defs.G_def
+  Simple_Network_Impl_nat_defs.W_def
+  Simple_Network_Impl_nat_defs.V_def
+  Simple_Network_Impl_nat_defs.E'_def
+  Simple_Network_Impl_nat_defs.E_def
+  Simple_Network_Impl_nat_defs.resets_def
+  Simple_Network_Impl_nat_defs.bound_def
+  Simple_Network_Impl_nat_defs.bound_inv_def
+  Simple_Network_Impl_nat_defs.bound_g_def
+  Simple_Network_Impl_nat_defs.collect_resets_def
+  Simple_Network_Impl_nat_defs.clkp_set''_def
+  Simple_Network_Impl_nat_defs.clkp_inv_def
+
+export_code Simple_Network_Impl_nat_defs.k checking SML_imp
+
+
+
+paragraph \<open>Calculating the Renaming\<close>
+
+definition "mem_assoc x = list_ex (\<lambda>(y, _). x = y)"
+
+definition "mk_renaming str xs \<equiv>
+do {
+  mapping \<leftarrow> fold_error
+    (\<lambda>x m.
+      if mem_assoc x m then Error [STR ''Duplicate name:'' + str x] else (x, length m) # m |> Result
+    ) xs [];
+  Result (the o map_of mapping)
+}"
+
+(* Unused *)
+lemma [simp]:
+  "is_result (make_err m e) \<longleftrightarrow> False"
+  by (cases e) auto
+
+(* Unused *)
+lemma is_result_assert_msg_iff[simp]:
+  "is_result (assert_msg b m r) \<longleftrightarrow> is_result r \<and> b"
+  unfolding assert_msg_def by simp
+
+(* Unused *)
+lemma
+  "is_result (e |> assert_msg b1 m |> assert_msg b2 m2) \<longleftrightarrow> is_result e \<and> b1 \<and> b2"
+  by simp
+
+
+context Simple_Network_Impl
+begin
+
+definition action_set where
+  "action_set \<equiv>
+    (\<Union>(_, trans, _) \<in> set automata. \<Union>(_, _, a, _, _, _) \<in> set trans. set_act a) \<union> set broadcast"
+
+definition loc_set' where
+  "loc_set' p = (\<Union>(l, _, _, _, _, l')\<in>set (fst (snd (automata ! p))). {l, l'})" for p
+
+end
+
+
+fun intersperse :: "'a \<Rightarrow> 'a list \<Rightarrow> 'a list" where
+  "intersperse sep (x # y # xs) = x # sep # intersperse sep (y # xs)" |
+  "intersperse _ xs = xs"
+
+definition
+  "concat_str = String.implode o concat o map String.explode"
+
+
+paragraph \<open>Unsafe Glue Code\<close>
+
+definition list_of_set :: "'a set \<Rightarrow> 'a list" where
+  "list_of_set xs = undefined"
+
+code_printing
+  constant list_of_set \<rightharpoonup> (SML) "(fn Set xs => xs) _"
+       and              (OCaml) "(fun x -> match x with Set xs -> xs) _"
+
+definition print :: "String.literal \<Rightarrow> unit" where
+  "print x = ()"
+
+code_printing
+  constant print \<rightharpoonup> (SML) "print _"
+       and        (OCaml) "print'_string _"
+
+definition println :: "String.literal \<Rightarrow> unit" where
+  "println x = print (x + STR ''\<newline>'')"
+
+definition "make_renaming \<equiv> \<lambda> broadcast automata bounds.
+  let
+    action_set = Simple_Network_Impl.action_set automata broadcast |> list_of_set;
+    clk_set = fst ` Simple_Network_Impl.clkp_set' automata |> list_of_set;
+    loc_set = (\<lambda>i. Simple_Network_Impl.loc_set' automata i |> list_of_set);
+    var_set = Prod_TA_Defs.var_set
+      (set broadcast, map Simple_Network_Impl.automaton_of automata, map_of bounds) |> list_of_set;
+    n_ps = length automata;
+    num_actions = length (remdups action_set);
+    m = length (remdups clk_set);
+    num_states_list = map (\<lambda>i. loc_set i |> remdups |> length) [0..<n_ps];
+    num_states = (\<lambda>i. num_states_list ! i);
+    mk_renaming = mk_renaming (\<lambda>x. x)
+  in do {
+    (renum_acts, renum_clocks, renum_vars) \<leftarrow>
+      mk_renaming action_set <|> mk_renaming clk_set <|> mk_renaming var_set;
+    renum_states_list \<leftarrow> combine_map (\<lambda>i. mk_renaming (loc_set i)) [0..<n_ps];
+    let renum_states = (\<lambda>i. renum_states_list ! i);
+    Result (m, num_states, num_actions, renum_acts, renum_vars, renum_clocks, renum_states)
+  }"
+
+definition "preproc_mc \<equiv> \<lambda> (broadcast, automata, bounds) L\<^sub>0 s\<^sub>0 formula.
+  case make_renaming broadcast automata bounds of
+    Error e \<Rightarrow> return (Error e)
+  | Result (m, num_states, num_actions, renum_acts, renum_vars, renum_clocks, renum_states) \<Rightarrow> do {
+    let (broadcast', automata', bounds') = rename_network
+      broadcast bounds automata renum_acts renum_vars renum_clocks renum_states;
+    let k = Simple_Network_Impl_nat_defs.k broadcast' bounds' automata' m num_states;
+    r \<leftarrow> rename_mc broadcast bounds automata k L\<^sub>0 s\<^sub>0 formula
+      m num_states num_actions renum_acts renum_vars renum_clocks renum_states;
+    return (Result r)
+  }
+"
+
+definition
+"main \<equiv> \<lambda> (broadcast, automata, bounds) L\<^sub>0 s\<^sub>0 formula. do {
+  r \<leftarrow> preproc_mc (broadcast, automata, bounds) L\<^sub>0 s\<^sub>0 formula;
+  return (case r of
+    Error es \<Rightarrow>
+      intersperse (STR ''\<newline>'') es
+      |> concat_str
+      |> (\<lambda>e. STR ''Error during preprocessing:\<newline>'' + e)
+      |> println
+  | Result Renaming_Failed \<Rightarrow> STR ''Renaming failed'' |> println
+  | Result Preconds_Unsat \<Rightarrow>  STR ''Input invalid'' |> println
+  | Result Unsat \<Rightarrow> STR ''Property is not satisfied!'' |> println
+  | Result Sat   \<Rightarrow> STR ''Property is satisfied!'' |> println
+  )
+}"
+
+lemmas [code] =
+  Simple_Network_Impl.action_set_def
+  Simple_Network_Impl.loc_set'_def
+
+export_code main in SML module_name Main
 
 end
